theories/program_logic/ectx_language.v
@@ -9,19 +9,19 @@ structure. Use the coercion [LanguageOfEctx] as defined in the bottom of this
 file for doing that. *)
 
 Section ectx_language_mixin.
-  Context {expr val ectx state observation : Type}.
+  Context {expr val ectx state : Type}.
   Context (of_val : val → expr).
   Context (to_val : expr → option val).
   Context (empty_ectx : ectx).
   Context (comp_ectx : ectx → ectx → ectx).
   Context (fill : ectx → expr → expr).
-  Context (head_step : expr → state → list observation → expr → state → list expr → Prop).
+  Context (head_step : expr → state → expr → state → list expr → Prop).
 
   Record EctxLanguageMixin := {
     mixin_to_of_val v : to_val (of_val v) = Some v;
     mixin_of_to_val e v : to_val e = Some v → of_val v = e;
-    mixin_val_head_stuck e1 σ1 κ e2 σ2 efs :
-      head_step e1 σ1 κ e2 σ2 efs → to_val e1 = None;
+    mixin_val_head_stuck e1 σ1 e2 σ2 efs :
+      head_step e1 σ1 e2 σ2 efs → to_val e1 = None;
 
     mixin_fill_empty e : fill empty_ectx e = e;
     mixin_fill_comp K1 K2 e : fill K1 (fill K2 e) = fill (comp_ectx K1 K2) e;
@@ -36,17 +36,17 @@ Section ectx_language_mixin.
 
         This implies there can be only one head redex, see
         [head_redex_unique]. *)
-    mixin_step_by_val K' K_redex e1' e1_redex σ1 κ e2 σ2 efs :
+    mixin_step_by_val K' K_redex e1' e1_redex σ1 e2 σ2 efs :
       fill K' e1' = fill K_redex e1_redex →
       to_val e1' = None →
-      head_step e1_redex σ1 κ e2 σ2 efs →
+      head_step e1_redex σ1 e2 σ2 efs →
       ∃ K'', K_redex = comp_ectx K' K'';
 
     (** If [fill K e] takes a head step, then either [e] is a value or [K] is
         the empty evaluation context. In other words, if [e] is not a value
         wrapping it in a context does not add new head redex positions. *)
-    mixin_head_ctx_step_val K e σ1 κ e2 σ2 efs :
-      head_step (fill K e) σ1 κ e2 σ2 efs → is_Some (to_val e) ∨ K = empty_ectx;
+    mixin_head_ctx_step_val K e σ1 e2 σ2 efs :
+      head_step (fill K e) σ1 e2 σ2 efs → is_Some (to_val e) ∨ K = empty_ectx;
   }.
 End ectx_language_mixin.
 
@@ -55,15 +55,14 @@ Structure ectxLanguage := EctxLanguage {
   val : Type;
   ectx : Type;
   state : Type;
-  observation : Type;
 
   of_val : val → expr;
   to_val : expr → option val;
   empty_ectx : ectx;
   comp_ectx : ectx → ectx → ectx;
   fill : ectx → expr → expr;
-  head_step : expr → state → list observation → expr → state → list expr → Prop;
-  config_step : state → list observation → state → Prop;
+  head_step : expr → state → expr → state → list expr → Prop;
+  config_step : state → state → Prop;
 
   ectx_language_mixin :
     EctxLanguageMixin of_val to_val empty_ectx comp_ectx fill head_step
@@ -72,14 +71,14 @@ Structure ectxLanguage := EctxLanguage {
 Bind Scope expr_scope with expr.
 Bind Scope val_scope with val.
 
-Arguments EctxLanguage {_ _ _ _ _ _ _ _ _ _ _} _ _.
+Arguments EctxLanguage {_ _ _ _ _ _ _ _ _ _} _ _.
 Arguments of_val {_} _.
 Arguments to_val {_} _.
 Arguments empty_ectx {_}.
 Arguments comp_ectx {_} _ _.
 Arguments fill {_} _ _.
-Arguments head_step {_} _ _ _ _ _ _.
-Arguments config_step {_} _ _ _.
+Arguments head_step {_} _ _ _ _ _.
+Arguments config_step {_} _ _.
 
 (* From an ectx_language, we can construct a language. *)
 Section ectx_language.
@@ -89,7 +88,7 @@ Section ectx_language.
   Implicit Types K : ectx Λ.
 
   (* Only project stuff out of the mixin that is not also in language *)
-  Lemma val_head_stuck e1 σ1 κ e2 σ2 efs : head_step e1 σ1 κ e2 σ2 efs → to_val e1 = None.
+  Lemma val_head_stuck e1 σ1 e2 σ2 efs : head_step e1 σ1 e2 σ2 efs → to_val e1 = None.
   Proof. apply ectx_language_mixin. Qed.
   Lemma fill_empty e : fill empty_ectx e = e.
   Proof. apply ectx_language_mixin. Qed.
@@ -99,22 +98,22 @@ Section ectx_language.
   Proof. apply ectx_language_mixin. Qed.
   Lemma fill_val K e : is_Some (to_val (fill K e)) → is_Some (to_val e).
   Proof. apply ectx_language_mixin. Qed.
-  Lemma step_by_val K' K_redex e1' e1_redex σ1 κ e2 σ2 efs :
+  Lemma step_by_val K' K_redex e1' e1_redex σ1 e2 σ2 efs :
       fill K' e1' = fill K_redex e1_redex →
       to_val e1' = None →
-      head_step e1_redex σ1 κ e2 σ2 efs →
+      head_step e1_redex σ1 e2 σ2 efs →
       ∃ K'', K_redex = comp_ectx K' K''.
   Proof. apply ectx_language_mixin. Qed.
-  Lemma head_ctx_step_val K e σ1 κ e2 σ2 efs :
-    head_step (fill K e) σ1 κ e2 σ2 efs → is_Some (to_val e) ∨ K = empty_ectx.
+  Lemma head_ctx_step_val K e σ1 e2 σ2 efs :
+    head_step (fill K e) σ1 e2 σ2 efs → is_Some (to_val e) ∨ K = empty_ectx.
   Proof. apply ectx_language_mixin. Qed.
 
   Definition head_reducible (e : expr Λ) (σ : state Λ) :=
-    ∃ κ e' σ' efs, head_step e σ κ e' σ' efs.
+    ∃ e' σ' efs, head_step e σ e' σ' efs.
   Definition head_reducible_no_obs (e : expr Λ) (σ : state Λ) :=
-    ∃ e' σ' efs, head_step e σ [] e' σ' efs.
+    ∃ e' σ' efs, head_step e σ e' σ' efs.
   Definition head_irreducible (e : expr Λ) (σ : state Λ) :=
-    ∀ κ e' σ' efs, ¬head_step e σ κ e' σ' efs.
+    ∀ e' σ' efs, ¬head_step e σ e' σ' efs.
   Definition head_stuck (e : expr Λ) (σ : state Λ) :=
     to_val e = None ∧ head_irreducible e σ.
 
@@ -123,14 +122,14 @@ Section ectx_language.
   Definition sub_redexes_are_values (e : expr Λ) :=
     ∀ K e', e = fill K e' → to_val e' = None → K = empty_ectx.
 
-  Inductive prim_step (e1 : expr Λ) (σ1 : state Λ) (κ : list (observation Λ))
+  Inductive prim_step (e1 : expr Λ) (σ1 : state Λ)
       (e2 : expr Λ) (σ2 : state Λ) (efs : list (expr Λ)) : Prop :=
     Ectx_step K e1' e2' :
       e1 = fill K e1' → e2 = fill K e2' →
-      head_step e1' σ1 κ e2' σ2 efs → prim_step e1 σ1 κ e2 σ2 efs.
+      head_step e1' σ1 e2' σ2 efs → prim_step e1 σ1 e2 σ2 efs.
 
-  Lemma Ectx_step' K e1 σ1 κ e2 σ2 efs :
-    head_step e1 σ1 κ e2 σ2 efs → prim_step (fill K e1) σ1 κ (fill K e2) σ2 efs.
+  Lemma Ectx_step' K e1 σ1 e2 σ2 efs :
+    head_step e1 σ1 e2 σ2 efs → prim_step (fill K e1) σ1 (fill K e2) σ2 efs.
   Proof. econstructor; eauto. Qed.
 
   Definition ectx_lang_mixin : LanguageMixin of_val to_val prim_step.
@@ -138,7 +137,7 @@ Section ectx_language.
     split.
     - apply ectx_language_mixin.
     - apply ectx_language_mixin.
-    - intros ?????? [??? -> -> ?%val_head_stuck].
+    - intros ????? [??? -> -> ?%val_head_stuck].
       apply eq_None_not_Some. by intros ?%fill_val%eq_None_not_Some.
   Qed.
 
@@ -146,14 +145,14 @@ Section ectx_language.
     Language config_step ectx_lang_mixin.
 
   Definition head_atomic (a : atomicity) (e : expr Λ) : Prop :=
-    ∀ σ κ e' σ' efs,
-      head_step e σ κ e' σ' efs →
+    ∀ σ e' σ' efs,
+      head_step e σ e' σ' efs →
       if a is WeaklyAtomic then irreducible e' σ' else is_Some (to_val e').
 
   Definition head_stutteringatomic (a : atomicity) (e : expr Λ) : Prop :=
-    ∀ σ κ e' σ' efs,
-      head_step e σ κ e' σ' efs →
-      (e' = e ∧ σ' = σ ∧ efs = [] ∧ κ = [])
+    ∀ σ e' σ' efs,
+      head_step e σ e' σ' efs →
+      (e' = e ∧ σ' = σ ∧ efs = [])
       ∨
       if a is WeaklyAtomic then irreducible e' σ' else is_Some (to_val e').
 
@@ -178,31 +177,31 @@ Section ectx_language.
     head_reducible e' σ →
     K = comp_ectx K' empty_ectx ∧ e = e'.
   Proof.
-    intros Heq (κ & e2 & σ2 & efs & Hred) (κ' & e2' & σ2' & efs' & Hred').
+    intros Heq (e2 & σ2 & efs & Hred) (e2' & σ2' & efs' & Hred').
     edestruct (step_by_val K' K e' e) as [K'' HK];
       [by eauto using val_head_stuck..|].
     subst K. move: Heq. rewrite -fill_comp. intros <-%(inj (fill _)).
-    destruct (head_ctx_step_val _ _ _ _ _ _ _ Hred') as [[]%not_eq_None_Some|HK''].
+    destruct (head_ctx_step_val _ _ _ _ _ _ Hred') as [[]%not_eq_None_Some|HK''].
     { by eapply val_head_stuck. }
     subst K''. rewrite fill_empty. done.
   Qed.
 
-  Lemma head_prim_step e1 σ1 κ e2 σ2 efs :
-    head_step e1 σ1 κ e2 σ2 efs → prim_step e1 σ1 κ e2 σ2 efs.
+  Lemma head_prim_step e1 σ1 e2 σ2 efs :
+    head_step e1 σ1 e2 σ2 efs → prim_step e1 σ1 e2 σ2 efs.
   Proof. apply Ectx_step with empty_ectx; by rewrite ?fill_empty. Qed.
 
-  Lemma head_step_not_stuck e σ κ e' σ' efs : head_step e σ κ e' σ' efs → not_stuck e σ.
+  Lemma head_step_not_stuck e σ e' σ' efs : head_step e σ e' σ' efs → not_stuck e σ.
   Proof. rewrite /not_stuck /reducible /=. eauto 10 using head_prim_step. Qed.
 
-  Lemma fill_prim_step K e1 σ1 κ e2 σ2 efs :
-    prim_step e1 σ1 κ e2 σ2 efs → prim_step (fill K e1) σ1 κ (fill K e2) σ2 efs.
+  Lemma fill_prim_step K e1 σ1 e2 σ2 efs :
+    prim_step e1 σ1 e2 σ2 efs → prim_step (fill K e1) σ1 (fill K e2) σ2 efs.
   Proof.
     destruct 1 as [K' e1' e2' -> ->].
     rewrite !fill_comp. by econstructor.
   Qed.
   Lemma fill_reducible K e σ : reducible e σ → reducible (fill K e) σ.
   Proof.
-    intros (κ&e'&σ'&efs&?). exists κ, (fill K e'), σ', efs.
+    intros (e'&σ'&efs&?). exists (fill K e'), σ', efs.
     by apply fill_prim_step.
   Qed.
   Lemma fill_reducible_no_obs K e σ : reducible_no_obs e σ → reducible_no_obs (fill K e) σ.
@@ -211,7 +210,7 @@ Section ectx_language.
     by apply fill_prim_step.
   Qed.
   Lemma head_prim_reducible e σ : head_reducible e σ → reducible e σ.
-  Proof. intros (κ&e'&σ'&efs&?). eexists κ, e', σ', efs. by apply head_prim_step. Qed.
+  Proof. intros (e'&σ'&efs&?). eexists e', σ', efs. by apply head_prim_step. Qed.
   Lemma head_prim_fill_reducible e K σ :
     head_reducible e σ → reducible (fill K e) σ.
   Proof. intro. by apply fill_reducible, head_prim_reducible. Qed.
@@ -228,7 +227,7 @@ Section ectx_language.
   Lemma prim_head_reducible e σ :
     reducible e σ → sub_redexes_are_values e → head_reducible e σ.
   Proof.
-    intros (κ&e'&σ'&efs&[K e1' e2' -> -> Hstep]) ?.
+    intros (e'&σ'&efs&[K e1' e2' -> -> Hstep]) ?.
     assert (K = empty_ectx) as -> by eauto 10 using val_head_stuck.
     rewrite fill_empty /head_reducible; eauto.
   Qed.
@@ -248,7 +247,7 @@ Section ectx_language.
   Lemma ectx_language_atomic a e :
     head_atomic a e → sub_redexes_are_values e → Atomic a e.
   Proof.
-    intros Hatomic_step Hatomic_fill σ κ e' σ' efs [K e1' e2' -> -> Hstep].
+    intros Hatomic_step Hatomic_fill σ e' σ' efs [K e1' e2' -> -> Hstep].
     assert (K = empty_ectx) as -> by eauto 10 using val_head_stuck.
     rewrite fill_empty. eapply Hatomic_step. by rewrite fill_empty.
   Qed.
@@ -256,18 +255,18 @@ Section ectx_language.
   Lemma ectx_language_stutteringatomic a e :
     head_stutteringatomic a e → sub_redexes_are_values e → StutteringAtomic a e.
   Proof.
-    intros Hatomic_step Hatomic_fill σ κ e' σ' efs [K e1' e2' -> -> Hstep].
+    intros Hatomic_step Hatomic_fill σ e' σ' efs [K e1' e2' -> -> Hstep].
     assert (K = empty_ectx) as -> by eauto 10 using val_head_stuck.
     revert Hatomic_step; rewrite !fill_empty; intros Hatomic_step.
     eapply Hatomic_step; done.
   Qed.
 
-  Lemma head_reducible_prim_step_ctx K e1 σ1 κ e2 σ2 efs :
+  Lemma head_reducible_prim_step_ctx K e1 σ1 e2 σ2 efs :
     head_reducible e1 σ1 →
-    prim_step (fill K e1) σ1 κ e2 σ2 efs →
-    ∃ e2', e2 = fill K e2' ∧ head_step e1 σ1 κ e2' σ2 efs.
+    prim_step (fill K e1) σ1 e2 σ2 efs →
+    ∃ e2', e2 = fill K e2' ∧ head_step e1 σ1 e2' σ2 efs.
   Proof.
-    intros (κ'&e2''&σ2''&efs''&HhstepK) [K' e1' e2' HKe1 -> Hstep].
+    intros (e2''&σ2''&efs''&HhstepK) [K' e1' e2' HKe1 -> Hstep].
     edestruct (step_by_val K) as [K'' ?];
       eauto using val_head_stuck; simplify_eq/=.
     rewrite -fill_comp in HKe1; simplify_eq.
@@ -277,10 +276,10 @@ Section ectx_language.
     by rewrite !fill_empty.
   Qed.
 
-  Lemma head_reducible_prim_step e1 σ1 κ e2 σ2 efs :
+  Lemma head_reducible_prim_step e1 σ1 e2 σ2 efs :
     head_reducible e1 σ1 →
-    prim_step e1 σ1 κ e2 σ2 efs →
-    head_step e1 σ1 κ e2 σ2 efs.
+    prim_step e1 σ1 e2 σ2 efs →
+    head_step e1 σ1 e2 σ2 efs.
   Proof.
     intros.
     edestruct (head_reducible_prim_step_ctx empty_ectx) as (?&?&?);
@@ -293,10 +292,10 @@ Section ectx_language.
   Proof.
     split; simpl.
     - eauto using fill_not_val.
-    - intros ?????? [K' e1' e2' Heq1 Heq2 Hstep].
+    - intros ????? [K' e1' e2' Heq1 Heq2 Hstep].
       by exists (comp_ectx K K') e1' e2'; rewrite ?Heq1 ?Heq2 ?fill_comp.
-    - intros e1 σ1 κ e2 σ2 efs Hnval [K'' e1'' e2'' Heq1 -> Hstep].
-      destruct (step_by_val K K'' e1 e1'' σ1 κ e2'' σ2 efs) as [K' ->]; eauto.
+    - intros e1 σ1 e2 σ2 efs Hnval [K'' e1'' e2'' Heq1 -> Hstep].
+      destruct (step_by_val K K'' e1 e1'' σ1 e2'' σ2 efs) as [K' ->]; eauto.
       rewrite -fill_comp in Heq1; apply (inj (fill _)) in Heq1.
       exists (fill K' e2''); rewrite -fill_comp; split; auto.
       econstructor; eauto.
@@ -304,8 +303,8 @@ Section ectx_language.
 
   Record pure_head_step (e1 e2 : expr Λ) := {
     pure_head_step_safe σ1 : head_reducible_no_obs e1 σ1;
-    pure_head_step_det σ1 κ e2' σ2 efs :
-      head_step e1 σ1 κ e2' σ2 efs → κ = [] ∧ σ2 = σ1 ∧ e2' = e2 ∧ efs = []
+    pure_head_step_det σ1 e2' σ2 efs :
+      head_step e1 σ1 e2' σ2 efs → σ2 = σ1 ∧ e2' = e2 ∧ efs = []
   }.
 
   Lemma pure_head_step_pure_step e1 e2 : pure_head_step e1 e2 → pure_step e1 e2.
@@ -313,7 +312,8 @@ Section ectx_language.
     intros [Hp1 Hp2]. split.
     - intros σ. destruct (Hp1 σ) as (e2' & σ2 & efs & ?).
       eexists e2', σ2, efs. by apply head_prim_step.
-    - intros σ1 κ e2' σ2 efs ?%head_reducible_prim_step; eauto using head_reducible_no_obs_reducible.
+    - intros σ1 e2' σ2 efs ?%head_reducible_prim_step;
+        eauto using head_reducible_no_obs_reducible.
   Qed.
 
   (** This is not an instance because HeapLang's [wp_pure] tactic already takes
@@ -338,7 +338,7 @@ work.
 Note that this trick no longer works when we switch to canonical projections
 because then the pattern match [let '...] will be desugared into projections. *)
 Definition LanguageOfEctx (Λ : ectxLanguage) : language :=
-  let '@EctxLanguage E V C St K of_val to_val empty comp fill head config mix := Λ in
-  @Language E V St K of_val to_val _ config
+  let '@EctxLanguage E V C St of_val to_val empty comp fill head config mix := Λ in
+  @Language E V St of_val to_val _ config
     (@ectx_lang_mixin
-       (@EctxLanguage E V C St K of_val to_val empty comp fill head config mix)).
+       (@EctxLanguage E V C St of_val to_val empty comp fill head config mix)).
