theories/program_logic/infinite_traces.v
@@ -38,25 +38,25 @@ Section inflist.
 
 End inflist.
 
-Definition inf_execution_trace Λ := inflist (list (observation Λ) * cfg Λ).
+Definition inf_execution_trace Λ := inflist (cfg Λ).
 
 Section inf_execution_trace.
   Context {Λ : language}.
 
-  Definition inf_exec_prepend (κ : list (observation Λ)) (c : cfg Λ)
+  Definition inf_exec_prepend (c : cfg Λ)
              (iex : inf_execution_trace Λ) : inf_execution_trace Λ :=
-    ((κ, c) :: iex)%inflist.
+    (c :: iex)%inflist.
 
   CoInductive valid_inf_exec :
     execution_trace Λ → inf_execution_trace Λ → Prop :=
   | valid_inf_exec_singleton ex :
       valid_exec ex → valid_inf_exec ex []%inflist
-  | valid_inf_exec_step ex c κ c' iex :
+  | valid_inf_exec_step ex c c' iex :
       valid_exec ex →
       exec_ends_in ex c →
-      step c κ c' →
-      valid_inf_exec (exec_extend ex κ c') iex →
-      valid_inf_exec ex (inf_exec_prepend κ c' iex).
+      step c c' →
+      valid_inf_exec (exec_extend ex c') iex →
+      valid_inf_exec ex (inf_exec_prepend c' iex).
 
 End inf_execution_trace.
 
@@ -72,16 +72,16 @@ CoInductive valid_inf_system_trace `{AS : AuxState Λ}
 | valid_system_trace_singleton ex atr :
     Ψ ex atr →
     valid_inf_system_trace Ψ ex atr []%inflist []%inflist
-| valid_system_trace_step ex atr c κ c' δ δ' iex iatr :
+| valid_system_trace_step ex atr c c' δ δ' iex iatr :
     Ψ ex atr →
     exec_ends_in ex c →
-    step c κ c' →
+    step c c' →
     auxtr_ends_in atr δ →
-    valid_state_evolution AS c.2 δ κ c'.2 δ' →
+    valid_state_evolution AS c.2 δ c'.2 δ' →
     valid_inf_system_trace
-      Ψ (exec_extend ex κ c') (auxtr_extend atr δ') iex iatr →
+      Ψ (exec_extend ex c') (auxtr_extend atr δ') iex iatr →
     valid_inf_system_trace
-      Ψ ex atr (inf_exec_prepend κ c' iex) (inf_auxtr_prepend δ' iatr).
+      Ψ ex atr (inf_exec_prepend c' iex) (inf_auxtr_prepend δ' iatr).
 
 Section simulation.
   Context {Λ : language} {AS : AuxState Λ}
@@ -90,21 +90,21 @@ Section simulation.
   Implicit Types ex : execution_trace Λ.
   Implicit Types iex : inf_execution_trace Λ.
 
-  Lemma valid_inf_exec_prepend_valid_exec_extend ex κ c iex :
-    valid_inf_exec ex (inf_exec_prepend κ c iex) →
-    valid_exec (exec_extend ex κ c).
+  Lemma valid_inf_exec_prepend_valid_exec_extend ex c iex :
+    valid_inf_exec ex (inf_exec_prepend c iex) →
+    valid_exec (exec_extend ex c).
   Proof.
-    inversion 1 as [|???????? Hex]; simplify_eq.
+    inversion 1 as [|??????? Hex]; simplify_eq.
     inversion Hex; done.
   Qed.
 
   Lemma produce_inf_aux_trace_next_aux_state_exists
         (ex : execution_trace Λ) (atr : auxiliary_trace AS)
         (Hcsm : continued_simulation φ ex atr)
-        (c : cfg Λ) (κ : list (observation Λ))
+        (c : cfg Λ)
         (iex : inf_execution_trace Λ)
-        (Hvex : valid_inf_exec ex (inf_exec_prepend κ c iex)) :
-    ∃ δ, continued_simulation φ (exec_extend ex κ c) (auxtr_extend atr δ).
+        (Hvex : valid_inf_exec ex (inf_exec_prepend c iex)) :
+    ∃ δ, continued_simulation φ (exec_extend ex c) (auxtr_extend atr δ).
   Proof.
     apply continued_simulation_next_aux_state_exists; first done.
     eapply valid_inf_exec_prepend_valid_exec_extend; eauto.
@@ -113,32 +113,32 @@ Section simulation.
   Definition produce_inf_aux_trace_next_aux_state
              (ex : execution_trace Λ) (atr : auxiliary_trace AS)
              (Hcsm : continued_simulation φ ex atr)
-             (c : cfg Λ) (κ : list (observation Λ))
+             (c : cfg Λ)
              (iex : inf_execution_trace Λ)
-             (Hvex : valid_inf_exec ex (inf_exec_prepend κ c iex))
+             (Hvex : valid_inf_exec ex (inf_exec_prepend c iex))
     : aux_state AS :=
     epsilon
-      (produce_inf_aux_trace_next_aux_state_exists ex atr Hcsm c κ iex Hvex).
+      (produce_inf_aux_trace_next_aux_state_exists ex atr Hcsm c iex Hvex).
 
   Lemma produce_inf_aux_trace_next_aux_state_continued_simulation
         (ex : execution_trace Λ) (atr : auxiliary_trace AS)
         (Hcsm : continued_simulation φ ex atr)
-        (c : cfg Λ) (κ : list (observation Λ))
+        (c : cfg Λ)
         (iex : inf_execution_trace Λ)
-        (Hvex : valid_inf_exec ex (inf_exec_prepend κ c iex)) :
+        (Hvex : valid_inf_exec ex (inf_exec_prepend c iex)) :
     continued_simulation
       φ
-      (exec_extend ex κ c)
+      (exec_extend ex c)
       (auxtr_extend
-         atr (produce_inf_aux_trace_next_aux_state ex atr Hcsm c κ iex Hvex)).
+         atr (produce_inf_aux_trace_next_aux_state ex atr Hcsm c iex Hvex)).
   Proof.
     rewrite /produce_inf_aux_trace_next_aux_state.
     apply epsilon_correct.
   Qed.
 
-  Local Lemma valid_inf_exec_adjust {ex c κ iex} :
-    valid_inf_exec ex ((κ, c) :: iex)%inflist →
-    valid_inf_exec (exec_extend ex κ c) iex.
+  Local Lemma valid_inf_exec_adjust {ex c iex} :
+    valid_inf_exec ex (c :: iex)%inflist →
+    valid_inf_exec (exec_extend ex c) iex.
   Proof. inversion 1; done. Qed.
 
   CoFixpoint produce_inf_aux_trace
@@ -149,16 +149,16 @@ Section simulation.
     inf_auxiliary_trace AS :=
     match iex as l return valid_inf_exec ex l → inf_auxiliary_trace AS with
     | [] => λ _, []
-    | (κ, c) :: iex' =>
+    | c :: iex' =>
       λ Hvex',
       let δ :=
-          produce_inf_aux_trace_next_aux_state ex atr Hcsm c κ iex' Hvex'
+          produce_inf_aux_trace_next_aux_state ex atr Hcsm c iex' Hvex'
       in
       δ :: (produce_inf_aux_trace
-              (exec_extend ex κ c)
+              (exec_extend ex c)
               (auxtr_extend atr δ)
               (produce_inf_aux_trace_next_aux_state_continued_simulation
-                 ex atr Hcsm c κ iex' Hvex')
+                 ex atr Hcsm c iex' Hvex')
               iex'
               (valid_inf_exec_adjust Hvex'))
     end%inflist Hvex.
@@ -175,12 +175,12 @@ Section simulation.
         (produce_inf_aux_trace ex atr Hcsm iex Hvex).
   Proof.
     revert ex atr Hcsm iex Hvex; cofix CIH; intros ex atr Hcsm iex Hvex.
-    destruct iex as [|[κ c] iex].
+    destruct iex as [|c iex].
     - rewrite [produce_inf_aux_trace _ _ _ _ _]inflist_unfold_fold /=.
       constructor; trivial.
     - rewrite [produce_inf_aux_trace _ _ _ _ _]inflist_unfold_fold /=.
       pose proof (produce_inf_aux_trace_next_aux_state_continued_simulation
-                    ex atr Hcsm c κ iex Hvex) as Hcsm'.
+                    ex atr Hcsm c iex Hvex) as Hcsm'.
       pose proof (continued_simulation_valid_system_trace _ _ _ Hcsm') as Hvst.
       apply valid_system_trace_extend_inv in Hvst as (?&?&?&?&?&?&?).
       econstructor; eauto.
