theories/aneris_lang/resources.v
@@ -15,12 +15,7 @@ Import Network.
 Record Model := model {
   model_state :> Type;
   model_rel :> model_state → model_state → Prop;
-  model_state_eq_dec : EqDecision model_state;
-  model_rel_proof_irrel : ∀ m m', ProofIrrel (model_rel m m');
-  model_rel_dec : ∀ m m', Decision (model_rel m m');
 }.
-
-Existing Instances model_state_eq_dec model_rel_proof_irrel model_rel_dec.
 
 Record node_gnames := Node_gname {
   heap_name : gname;
