theories/program_logic/ectx_lifting.v
@@ -19,16 +19,16 @@ Hint Resolve head_stuck_stuck : core.
 
 Lemma wp_lift_head_step_fupd {s E Φ} e1 :
   to_val e1 = None →
-  (∀ σ1 δ1 κ κs n, state_interp σ1 δ1 κs n ={E,∅}=∗
+  (∀ σ1 δ1 n, state_interp σ1 δ1 n ={E,∅}=∗
     ⌜head_reducible e1 σ1⌝ ∗
-    ∀ e2 σ2 efs, ⌜head_step e1 σ1 κ e2 σ2 efs⌝ ={∅}=∗ ▷ |={∅,E}=>
-      ∃ δ2, ⌜valid_state_evolution AS σ1 δ1 κ σ2 δ2⌝ ∗
-      state_interp σ2 δ2 (κs ++ κ) (length efs + n) ∗
+    ∀ e2 σ2 efs, ⌜head_step e1 σ1 e2 σ2 efs⌝ ={∅}=∗ ▷ |={∅,E}=>
+      ∃ δ2, ⌜valid_state_evolution AS σ1 δ1 σ2 δ2⌝ ∗
+      state_interp σ2 δ2 (length efs + n) ∗
       WP e2 @ s; E {{ Φ }} ∗
       [∗ list] ef ∈ efs, WP ef @ s; ⊤ {{ fork_post }})
   ⊢ WP e1 @ s; E {{ Φ }}.
 Proof.
-  iIntros (?) "H". iApply wp_lift_step_fupd=>//. iIntros (σ1 κ κs Qs st) "Hσ".
+  iIntros (?) "H". iApply wp_lift_step_fupd=>//. iIntros (σ1 Qs st) "Hσ".
   iMod ("H" with "Hσ") as "[% H]"; iModIntro.
   iSplit; first by destruct s; eauto. iIntros (e2 σ2 efs ?).
   iApply "H"; eauto.
@@ -36,16 +36,16 @@ Qed.
 
 Lemma wp_lift_head_step {s E Φ} e1 :
   to_val e1 = None →
-  (∀ σ1 δ1 κ κs n, state_interp σ1 δ1 κs n ={E,∅}=∗
+  (∀ σ1 δ1 n, state_interp σ1 δ1 n ={E,∅}=∗
     ⌜head_reducible e1 σ1⌝ ∗
-    ▷ ∀ e2 σ2 efs, ⌜head_step e1 σ1 κ e2 σ2 efs⌝ ={∅,E}=∗
-      ∃ δ2, ⌜valid_state_evolution AS σ1 δ1 κ σ2 δ2⌝ ∗
-      state_interp σ2 δ2 (κs ++ κ) (length efs + n) ∗
+    ▷ ∀ e2 σ2 efs, ⌜head_step e1 σ1 e2 σ2 efs⌝ ={∅,E}=∗
+      ∃ δ2, ⌜valid_state_evolution AS σ1 δ1 σ2 δ2⌝ ∗
+      state_interp σ2 δ2 (length efs + n) ∗
       WP e2 @ s; E {{ Φ }} ∗
       [∗ list] ef ∈ efs, WP ef @ s; ⊤ {{ fork_post }})
   ⊢ WP e1 @ s; E {{ Φ }}.
 Proof.
-  iIntros (?) "H". iApply wp_lift_head_step_fupd; [done|]. iIntros (?????) "?".
+  iIntros (?) "H". iApply wp_lift_head_step_fupd; [done|]. iIntros (???) "?".
   iMod ("H" with "[$]") as "[$ H]". iIntros "!>" (e2 σ2 efs ?) "!> !>".
   iApply "H"; done.
 Qed.
@@ -53,11 +53,11 @@ Qed.
 Lemma wp_lift_head_stuck E Φ e :
   to_val e = None →
   sub_redexes_are_values e →
-  (∀ σ κs n st, state_interp σ κs n st ={E,∅}=∗ ⌜head_stuck e σ⌝)
+  (∀ σ n st, state_interp σ n st ={E,∅}=∗ ⌜head_stuck e σ⌝)
   ⊢ WP e @ E ?{{ Φ }}.
 Proof.
   iIntros (??) "H". iApply wp_lift_stuck; first done.
-  iIntros (σ κs n st) "Hσ". iMod ("H" with "Hσ") as "%". by auto.
+  iIntros (σ n st) "Hσ". iMod ("H" with "Hσ") as "%". by auto.
 Qed.
 
 Lemma wp_lift_pure_head_stuck E Φ e :
@@ -67,56 +67,56 @@ Lemma wp_lift_pure_head_stuck E Φ e :
   ⊢ WP e @ E ?{{ Φ }}.
 Proof using Hinh.
   iIntros (?? Hstuck). iApply wp_lift_head_stuck; [done|done|].
-  iIntros (σ κs n st) "_". iMod (fupd_mask_subseteq ∅) as "_"; first set_solver.
+  iIntros (σ n st) "_". iMod (fupd_mask_subseteq ∅) as "_"; first set_solver.
   auto; done.
 Qed.
 
 Lemma wp_lift_atomic_head_step_fupd {s E1 E2 Φ} e1 :
   to_val e1 = None →
-  (∀ σ1 δ1 κ κs n, state_interp σ1 δ1 κs n ={E1}=∗
+  (∀ σ1 δ1 n, state_interp σ1 δ1 n ={E1}=∗
     ⌜head_reducible e1 σ1⌝ ∗
-    ∀ e2 σ2 efs, ⌜head_step e1 σ1 κ e2 σ2 efs⌝ ={E1}[E2]▷=∗
-      ∃ δ2, ⌜valid_state_evolution AS σ1 δ1 κ σ2 δ2⌝ ∗
-      state_interp σ2 δ2 (κs ++ κ) (length efs + n) ∗
+    ∀ e2 σ2 efs, ⌜head_step e1 σ1 e2 σ2 efs⌝ ={E1}[E2]▷=∗
+      ∃ δ2, ⌜valid_state_evolution AS σ1 δ1 σ2 δ2⌝ ∗
+      state_interp σ2 δ2 (length efs + n) ∗
       from_option Φ False (to_val e2) ∗
       [∗ list] ef ∈ efs, WP ef @ s; ⊤ {{ fork_post }})
   ⊢ WP e1 @ s; E1 {{ Φ }}.
 Proof.
   iIntros (?) "H". iApply wp_lift_atomic_step_fupd; [done|].
-  iIntros (σ1 κ κs Qs st) "Hσ1". iMod ("H" with "Hσ1") as "[% H]"; iModIntro.
+  iIntros (σ1 Qs st) "Hσ1". iMod ("H" with "Hσ1") as "[% H]"; iModIntro.
   iSplit; first by destruct s; auto. iIntros (e2 σ2 efs Hstep).
   iApply "H"; eauto.
 Qed.
 
 Lemma wp_lift_atomic_head_step {s E Φ} e1 :
   to_val e1 = None →
-  (∀ σ1 δ1 κ κs n, state_interp σ1 δ1 κs n ={E}=∗
+  (∀ σ1 δ1 n, state_interp σ1 δ1 n ={E}=∗
     ⌜head_reducible e1 σ1⌝ ∗
-    ▷ ∀ e2 σ2 efs, ⌜head_step e1 σ1 κ e2 σ2 efs⌝ ={E}=∗
-      ∃ δ2, ⌜valid_state_evolution AS σ1 δ1 κ σ2 δ2⌝ ∗
-      state_interp σ2 δ2 (κs ++ κ) (length efs + n) ∗
+    ▷ ∀ e2 σ2 efs, ⌜head_step e1 σ1 e2 σ2 efs⌝ ={E}=∗
+      ∃ δ2, ⌜valid_state_evolution AS σ1 δ1 σ2 δ2⌝ ∗
+      state_interp σ2 δ2 (length efs + n) ∗
       from_option Φ False (to_val e2) ∗
       [∗ list] ef ∈ efs, WP ef @ s; ⊤ {{ fork_post }})
   ⊢ WP e1 @ s; E {{ Φ }}.
 Proof.
   iIntros (?) "H". iApply wp_lift_atomic_step; eauto.
-  iIntros (σ1 κ κs Qs st) "Hσ1". iMod ("H" with "Hσ1") as "[% H]"; iModIntro.
+  iIntros (σ1 Qs st) "Hσ1". iMod ("H" with "Hσ1") as "[% H]"; iModIntro.
   iSplit; first by destruct s; auto. iNext. iIntros (e2 σ2 efs Hstep).
   iApply "H"; eauto.
 Qed.
 
 Lemma wp_lift_atomic_head_step_no_fork_fupd {s E1 E2 Φ} e1 :
   to_val e1 = None →
-  (∀ σ1 δ1 κ κs n, state_interp σ1 δ1 κs n ={E1}=∗
+  (∀ σ1 δ1 n, state_interp σ1 δ1 n ={E1}=∗
     ⌜head_reducible e1 σ1⌝ ∗
-    ∀ e2 σ2 efs, ⌜head_step e1 σ1 κ e2 σ2 efs⌝ ={E1}[E2]▷=∗
-      ∃ δ2, ⌜valid_state_evolution AS σ1 δ1 κ σ2 δ2⌝ ∗
-      ⌜efs = []⌝ ∗ state_interp σ2 δ2 (κs ++ κ) n ∗
+    ∀ e2 σ2 efs, ⌜head_step e1 σ1 e2 σ2 efs⌝ ={E1}[E2]▷=∗
+      ∃ δ2, ⌜valid_state_evolution AS σ1 δ1 σ2 δ2⌝ ∗
+      ⌜efs = []⌝ ∗ state_interp σ2 δ2 n ∗
       from_option Φ False (to_val e2))
   ⊢ WP e1 @ s; E1 {{ Φ }}.
 Proof.
   iIntros (?) "H". iApply wp_lift_atomic_head_step_fupd; [done|].
-  iIntros (σ1 κ κs Qs st) "Hσ1".
+  iIntros (σ1 Qs st) "Hσ1".
   iMod ("H" $! σ1 with "Hσ1") as "[$ H]"; iModIntro.
   iIntros (v2 σ2 efs Hstep).
   iMod ("H" $! v2 σ2 efs with "[# //]") as "H".
@@ -127,16 +127,16 @@ Qed.
 
 Lemma wp_lift_atomic_head_step_no_fork {s E Φ} e1 :
   to_val e1 = None →
-  (∀ σ1 δ1 κ κs n, state_interp σ1 δ1 κs n ={E}=∗
+  (∀ σ1 δ1 n, state_interp σ1 δ1 n ={E}=∗
     ⌜head_reducible e1 σ1⌝ ∗
-    ▷ ∀ e2 σ2 efs, ⌜head_step e1 σ1 κ e2 σ2 efs⌝ ={E}=∗
-      ∃ δ2, ⌜valid_state_evolution AS σ1 δ1 κ σ2 δ2⌝ ∗
-      ⌜efs = []⌝ ∗ state_interp σ2 δ2 (κs ++ κ) n ∗
+    ▷ ∀ e2 σ2 efs, ⌜head_step e1 σ1 e2 σ2 efs⌝ ={E}=∗
+      ∃ δ2, ⌜valid_state_evolution AS σ1 δ1 σ2 δ2⌝ ∗
+      ⌜efs = []⌝ ∗ state_interp σ2 δ2 n ∗
       from_option Φ False (to_val e2))
   ⊢ WP e1 @ s; E {{ Φ }}.
 Proof.
   iIntros (?) "H". iApply wp_lift_atomic_head_step; eauto.
-  iIntros (σ1 κ κs Qs st) "Hσ1".
+  iIntros (σ1 Qs st) "Hσ1".
   iMod ("H" $! σ1 with "Hσ1") as "[$ H]"; iModIntro.
   iNext; iIntros (v2 σ2 efs Hstep).
   iMod ("H" $! v2 σ2 efs with "[//]") as (st') "(% & -> & ? & ?) /=".
@@ -147,8 +147,8 @@ Qed.
 Lemma wp_lift_pure_det_head_step_no_fork {s E E' Φ} e1 e2 :
   to_val e1 = None →
   (∀ σ1, head_reducible e1 σ1) →
-  (∀ σ1 κ e2' σ2 efs',
-    head_step e1 σ1 κ e2' σ2 efs' → κ = [] ∧ σ2 = σ1 ∧ e2' = e2 ∧ efs' = []) →
+  (∀ σ1 e2' σ2 efs',
+    head_step e1 σ1 e2' σ2 efs' → σ2 = σ1 ∧ e2' = e2 ∧ efs' = []) →
   (|={E}[E']▷=> WP e2 @ s; E {{ Φ }}) ⊢ WP e1 @ s; E {{ Φ }}.
 Proof using Hinh.
   intros. rewrite -(wp_lift_pure_det_step_no_fork e1 e2); eauto.
@@ -158,8 +158,8 @@ Qed.
 Lemma wp_lift_pure_det_head_step_no_fork' {s E Φ} e1 e2 :
   to_val e1 = None →
   (∀ σ1, head_reducible e1 σ1) →
-  (∀ σ1 κ e2' σ2 efs',
-    head_step e1 σ1 κ e2' σ2 efs' → κ = [] ∧ σ2 = σ1 ∧ e2' = e2 ∧ efs' = []) →
+  (∀ σ1 e2' σ2 efs',
+    head_step e1 σ1 e2' σ2 efs' → σ2 = σ1 ∧ e2' = e2 ∧ efs' = []) →
   ▷ WP e2 @ s; E {{ Φ }} ⊢ WP e1 @ s; E {{ Φ }}.
 Proof using Hinh.
   intros. rewrite -[(WP e1 @ s; _ {{ _ }})%I]wp_lift_pure_det_head_step_no_fork //.
