theories/program_logic/ectxi_language.v
@@ -26,17 +26,17 @@ Below you can find the relevant parts:
 *)
 
 Section ectxi_language_mixin.
-  Context {expr val ectx_item state observation : Type}.
+  Context {expr val ectx_item state : Type}.
   Context (of_val : val → expr).
   Context (to_val : expr → option val).
   Context (fill_item : ectx_item → expr → expr).
-  Context (head_step : expr → state → list observation → expr → state → list expr → Prop).
-  Context (config_step : state → list observation → state → Prop).
+  Context (head_step : expr → state → expr → state → list expr → Prop).
+  Context (config_step : state → state → Prop).
 
   Record EctxiLanguageMixin := {
     mixin_to_of_val v : to_val (of_val v) = Some v;
     mixin_of_to_val e v : to_val e = Some v → of_val v = e;
-    mixin_val_stuck e1 σ1 κ e2 σ2 efs : head_step e1 σ1 κ e2 σ2 efs → to_val e1 = None;
+    mixin_val_stuck e1 σ1 e2 σ2 efs : head_step e1 σ1 e2 σ2 efs → to_val e1 = None;
 
     mixin_fill_item_val Ki e : is_Some (to_val (fill_item Ki e)) → is_Some (to_val e);
     (** [fill_item] is always injective on the expression for a fixed
@@ -52,8 +52,8 @@ Section ectxi_language_mixin.
         [ectx_language], an empty context is impossible here).  In other words,
         if [e] is not a value then wrapping it in a context does not add new
         head redex positions. *)
-    mixin_head_ctx_step_val Ki e σ1 κ e2 σ2 efs :
-      head_step (fill_item Ki e) σ1 κ e2 σ2 efs → is_Some (to_val e);
+    mixin_head_ctx_step_val Ki e σ1 e2 σ2 efs :
+      head_step (fill_item Ki e) σ1 e2 σ2 efs → is_Some (to_val e);
   }.
 End ectxi_language_mixin.
 
@@ -62,13 +62,12 @@ Structure ectxiLanguage := EctxiLanguage {
   val : Type;
   ectx_item : Type;
   state : Type;
-  observation : Type;
 
   of_val : val → expr;
   to_val : expr → option val;
   fill_item : ectx_item → expr → expr;
-  head_step : expr → state → list observation → expr → state → list expr → Prop;
-  config_step : state → list observation → state → Prop;
+  head_step : expr → state → expr → state → list expr → Prop;
+  config_step : state → state → Prop;
 
   ectxi_language_mixin :
     EctxiLanguageMixin of_val to_val fill_item head_step
@@ -77,12 +76,12 @@ Structure ectxiLanguage := EctxiLanguage {
 Bind Scope expr_scope with expr.
 Bind Scope val_scope with val.
 
-Arguments EctxiLanguage {_ _ _ _ _ _ _ _ _} _ _.
+Arguments EctxiLanguage {_ _ _ _ _ _ _ _} _ _.
 Arguments of_val {_} _.
 Arguments to_val {_} _.
 Arguments fill_item {_} _ _.
-Arguments head_step {_} _ _ _ _ _ _.
-Arguments config_step {_} _ _ _.
+Arguments head_step {_} _ _ _ _ _.
+Arguments config_step {_} _ _.
 
 Section ectxi_language.
   Context {Λ : ectxiLanguage}.
@@ -98,8 +97,8 @@ Section ectxi_language.
     to_val e1 = None → to_val e2 = None →
     fill_item Ki1 e1 = fill_item Ki2 e2 → Ki1 = Ki2.
   Proof. apply ectxi_language_mixin. Qed.
-  Lemma head_ctx_step_val Ki e σ1 κ e2 σ2 efs :
-    head_step (fill_item Ki e) σ1 κ e2 σ2 efs → is_Some (to_val e).
+  Lemma head_ctx_step_val Ki e σ1 e2 σ2 efs :
+    head_step (fill_item Ki e) σ1 e2 σ2 efs → is_Some (to_val e).
   Proof. apply ectxi_language_mixin. Qed.
 
   Definition fill (K : ectx) (e : expr Λ) : expr Λ := foldl (flip fill_item) e K.
@@ -122,7 +121,7 @@ Section ectxi_language.
     - intros K1 K2 e. by rewrite /fill /= foldl_app.
     - intros K; induction K as [|Ki K IH]; rewrite /Inj; naive_solver.
     - done.
-    - intros K K' e1 κ e1' σ1 e2 σ2 efs Hfill Hred Hstep; revert K' Hfill.
+    - intros K K' e1 e1' σ1 e2 σ2 efs Hfill Hred Hstep; revert K' Hfill.
       induction K as [|Ki K IH] using rev_ind=> /= K' Hfill; eauto using app_nil_r.
       destruct K' as [|Ki' K' _] using @rev_ind; simplify_eq/=.
       { rewrite fill_app in Hstep. apply head_ctx_step_val in Hstep.
@@ -133,7 +132,7 @@ Section ectxi_language.
         apply fill_not_val. revert Hstep. apply ectxi_language_mixin. }
       simplify_eq. destruct (IH K') as [K'' ->]; auto.
       exists K''. by rewrite assoc.
-    - intros K e1 σ1 κ e2 σ2 efs.
+    - intros K e1 σ1 e2 σ2 efs.
       destruct K as [|Ki K _] using rev_ind; simpl; first by auto.
       rewrite fill_app /=.
       intros ?%head_ctx_step_val; eauto using fill_val.
@@ -163,7 +162,7 @@ Coercion ectxi_lang_ectx : ectxiLanguage >-> ectxLanguage.
 Coercion ectxi_lang : ectxiLanguage >-> language.
 
 Definition EctxLanguageOfEctxi (Λ : ectxiLanguage) : ectxLanguage :=
-  let '@EctxiLanguage E V C St K of_val to_val fill head config mix := Λ in
-  @EctxLanguage E V (list C) St K of_val to_val _ _ _ _ config
+  let '@EctxiLanguage E V C St of_val to_val fill head config mix := Λ in
+  @EctxLanguage E V (list C) St of_val to_val _ _ _ _ config
     (@ectxi_lang_ectx_mixin
-       (@EctxiLanguage E V C St K of_val to_val fill head config mix)).
+       (@EctxiLanguage E V C St of_val to_val fill head config mix)).
